\subsection{Завдання 4: (Знайти траєкторію)}

$\left\{\begin{aligned}
    \frac{dy}{dt} &= -2\gamma y - \omega_0^2x \\
    \frac{dx}{dt} &= y
\end{aligned}\right.$

$\frac{dy}{dx} = -2\gamma - \omega^2_0 \frac{x}{y} \ \ \Bigg | \ y = xz, \ dy = zdx + xdz$

$z + x\frac{dz}{dx} = -2\gamma - \frac{\omega_0^2}{z}$

$-\frac{dx}{x} = \frac{dz}{z + 2\gamma + \frac{\omega_0^2}{z}} \ \ \Bigg | \cdot \frac{z}{z}$

$-\frac{dx}{x} = \frac{zdz}{z^2 + 2\gamma z + \omega_0^2} = 
\frac{zdz}{(z^2 + 2\gamma z + \gamma ^2) - (\gamma^2 - \omega_0^2)} \ \ \Bigg | \Delta =  \gamma^2 - \omega_0^2$

$-\frac{dx}{x} = \frac{zdz}{(z + \gamma)^2 - \Delta} = 
\frac{(z + \gamma - \gamma)d(z+\gamma)}{(z + \gamma)^2 - \Delta} = 
\frac{(z + \gamma)d(z+\gamma)}{(z + \gamma)^2 - \Delta} - \gamma\frac{d(z+\gamma)}{(z + \gamma)^2 - \Delta}$

$-\frac{dx}{x} = \frac{1}{2}\frac{d((z+\gamma)^2 - \Delta)}{(z + \gamma)^2 - \Delta} - \gamma\frac{d(z+\gamma)}{(z + \gamma)^2 - \Delta}$

\begin{equation} \label{pr3:eq8}
    -\ln x = \frac{1}{2} \ln {((z+\gamma)^2 - \Delta)} - \gamma \int \frac{d(z+\gamma)}{(z + \gamma)^2 - \Delta} + \ln C_0
\end{equation}


% $\Bigg [ \frac{d(z+\gamma)}{(z + \gamma)^2 - \Delta}  = \Big | p = z + \gamma, \ dp = d(z+\gamma) \ \Big | = 
% \frac{dp}{p^2 - \Delta} = \frac{dp}{(p + \sqrt{\Delta})(p - \sqrt{\Delta})}  = 
% \Big [ \frac{A}{p + \sqrt{\Delta}} + \frac{B}{p - \sqrt{\Delta}} = \frac{Ap - A\sqrt{\Delta} + Bp + B\sqrt{\Delta}}{(p + \sqrt{\Delta})(p - \sqrt{\Delta})}  =\\
%  = \left\{\begin{aligned}
%     B - A = 1\\
%     B + A = 0
% \end{aligned}\right. \Longrightarrow \ B = \frac{1}{2}, \ \ A = -\frac{1}{2} \Big ] = 
% \frac{1}{2} \Big (\frac{dp}{p + \sqrt{\Delta}} - \frac{dp}{p - \sqrt{\Delta}}\Big) = \frac{1}{2}\Big(\frac{d(z-\gamma)}{(z-\gamma) + \sqrt{\Delta}} - \frac{d(z-\gamma)}{(z-\gamma) - \sqrt{\Delta}}\Big) \Bigg ]$


% отже рівність (\ref{pr3:eq8}) приймає вигляд 

% $\ln x^2 + \ln {((z+\gamma)^2 - \Delta)} = \gamma \ln\frac{(z+\gamma) + \sqrt{\Delta}}{(z+\gamma) - \sqrt{\Delta}} + C_1$

Нехай $\Delta < 0$ тоді  (\ref{pr3:eq8}) матиме вигляд 

$-\ln x = \frac{1}{2} \ln {((z+\gamma)^2 + |\Delta|)} - \gamma \int \frac{d(z+\gamma)}{(z + \gamma)^2 + |\Delta|} + \ln C_0$

$-\ln x = \frac{1}{2} \ln {((z+\gamma)^2 + \Delta)} - \frac{\gamma}{\sqrt{|\Delta|}} \arctg \frac{z+\gamma}{\sqrt{|\Delta|}}+ \ln C$

$\ln x^2((z+\gamma)^2 +|\Delta|) = \frac{2\gamma}{\sqrt{|\Delta|}} \arctg \frac{z+\gamma}{\sqrt{|\Delta|}} - \ln C^2$

$\ln ( x^2z^2+x^2\gamma z + \gamma^2 - \gamma^2 + \omega_0^2) = \frac{2\gamma}{\omega} \arctg \frac{z+\gamma}{\omega} - \ln C^2$

\begin{equation}
    \ln ( y^2+\gamma xy + \omega_0^2 x^2) = \frac{2\gamma}{\omega} \arctg \frac{y+\gamma x}{\omega x} - \ln C^2
\end{equation}

% Нехай $\Delta > 0, \gamma > \omega_0$ тоді  (\ref{pr3:eq8}) матиме вигляд

% $-\frac{dx}{x} = \frac{zdz}{z^2 + 2\gamma z + \omega_0^2} = 
% \frac{zdz}{(z-(-\gamma+\sqrt{\Delta}))(z-(-\gamma-\sqrt{\Delta}))} = 
% \frac{zdz}{(z-\lambda_1)(z-\lambda_2)} = \Big| \frac{A}{z-\lambda_1} + \frac{B}{z-\lambda_2} \Longrightarrow\\ \Longrightarrow
% \left\{\begin{aligned}
%     &\lambda_2 A + \lambda_1 B = 0\\
%     &A + B = 1
% \end{aligned}\right. \Longrightarrow 
% \left\{\begin{aligned}
%     &\lambda_2 (1-B) + \lambda_1 B = 0\\
%     &A = 1 - B
% \end{aligned}\right. \Longrightarrow 
% \left\{\begin{aligned}
%     A = \frac{-\lambda_1}{\lambda_2 - \lambda_1}\\
%     B = \frac{\lambda_2}{\lambda_2 - \lambda_1}
% \end{aligned}\right| \Longrightarrow \\ \Longrightarrow
% -\frac{dx}{x} =  \frac{\lambda_2}{\lambda_2 - \lambda_1}\frac{dz}{z-\lambda_2} - 
% \frac{\lambda_1}{\lambda_2 - \lambda_1} \frac{dz}{z-\lambda_1}$

% $\ln|x| =  -\frac{\lambda_2}{\lambda_2 - \lambda_1}\ln|z-\lambda_2| + 
% \frac{\lambda_1}{\lambda_2 - \lambda_1} \ln|z-\lambda_1|$