\subsection{Завдання 5:}

$\ddot{x} + 2\gamma\dot{x}+\omega_0^2x = 0 \ \Longrightarrow \ 
\left\{\begin{aligned}
    \frac{dy}{dt} &= -2\gamma y -\omega_0^2x\\
    \frac{dx}{dt} &= y 
\end{aligned}\right.$

\begin{figure}[ht]
    \begin{minipage}[h]{0.49\linewidth}
        \input{practices/1_pr/source/pr1_4.tex} \\
        \centering {a)}
    \end{minipage}
    \begin{minipage}[h]{0.49\linewidth}
        \input{practices/1_pr/source/pr1_5.tex} \\
        \centering{b)}
    \end{minipage}
\end{figure}

\textbf{Знайти $\Gamma$}

$\dive \overrightarrow{V} = -2\gamma$

$\ln \Gamma = -2\gamma t + C$

$\Gamma(t) = \Gamma(0)e^{-2\gamma t}$

\textbf{Записати в полярних координатах}

$\left\{\begin{aligned}
    \frac{dy}{dt} &= -2\gamma y -\omega_0^2x\\
    \frac{dx}{dt} &= y 
\end{aligned}\right.$

$\left\{\begin{aligned}
    x = r\cos \varphi \\
    y = r\sin \varphi 
\end{aligned}\right.$

$\left\{\begin{aligned}
    \dot{r}\sin \varphi + \dot{\varphi}r \cos \varphi &=  -2\gamma r\sin \varphi - \omega_0^2 r\cos \varphi \ \ (*)\\
    \dot{r}\cos \varphi - \dot{\varphi} r \sin \varphi &= r \sin \varphi \ \ (**)
\end{aligned}\right.$

$\dot{r}:\ \ (*) \sin\varphi + (**)\cos\varphi \Longrightarrow \dot{r} = -2\gamma r\sin^2 \varphi - \omega_0^2 r\cos \varphi\sin\varphi + r\sin\varphi\cos\varphi =\\
= (1-\omega^2_0)r\cos\varphi\sin\varphi - 2\gamma r\sin^2\varphi $

$\dot{\varphi}:\ \ (*) \cos\varphi + (**)(-\sin\varphi) \Longrightarrow \dot{\varphi}r = -2\gamma r\sin \varphi\cos\varphi -\omega_0^2 r\cos^2\varphi - r\sin^2\varphi$

$\left\{\begin{aligned}
    \dot{r} &= (1-\omega^2_0)r\cos\varphi\sin\varphi - 2\gamma r\sin^2\varphi\\
    \dot{\varphi} &= -2\gamma \sin \varphi\cos\varphi -\omega_0^2 \cos^2\varphi - \sin^2\varphi
\end{aligned}\right.$

% $\left\{\begin{aligned}
%     -\dot{r} &= \dot{\varphi}r\ctg \varphi + 2\gamma r + \omega_0^2 r \ctg \varphi \\
%     \dot{\varphi} &= \frac{\dot{r}\ctg \varphi }{r} - 1
% \end{aligned}\right.$

% $-\dot{\varphi} = \dot{\varphi} \ctg^2 \varphi + 2\gamma\ctg \varphi + \omega_0^2 \ctg^2 \varphi + 1$

% $-\dot{\varphi}(1 + \ctg^2\varphi) =  2\gamma\ctg \varphi + \omega_0^2 \ctg^2\varphi + 1\ | \ 1+\ctg^2\varphi = \frac{1}{\sin^2\varphi}$ 

% $\dot{\varphi} = -2\gamma\cos\varphi\sin\varphi - \omega^2_0\cos^2\varphi - \sin^2\varphi= 
% -\gamma\sin 2\varphi - \omega_0^2\cos^2\varphi - \sin^2\varphi \ldots$ 

% \textcolor{red}{Потрібно доробити}